sledge/semantics/memory_modelScript.sml
@@ -1,0 +1,570 @@
+(*
+ * Copyright (c) Facebook, Inc. and its affiliates.
+ *
+ * This source code is licensed under the MIT license found in the
+ * LICENSE file in the root directory of this source tree.
+ *)
+
+(* A simple, concrete memory model where the heap is an array of bytes. This is
+ * how llair views memory, and how we give semantics to llvm. Although LLVM's
+ * real memory model is still a subject of research, this is mostly to do with
+ * enabling the right collection of compiler optimisations. Since we only want to
+ * think about LLVM semantics after optimisation, the concrete model is likely to
+ * be sufficient. *)
+
+open HolKernel boolLib bossLib Parse;
+open arithmeticTheory listTheory rich_listTheory pairTheory;
+open logrootTheory numposrepTheory wordsTheory pred_setTheory finite_mapTheory;
+open settingsTheory miscTheory;
+
+new_theory "memory_model";
+
+numLib.prefer_num ();
+
+(* Heap addresses *)
+Datatype:
+  addr = A num
+End
+
+(* Values that fit in registers *)
+Datatype:
+  reg_v =
+  | FlatV 'a
+  | AggV (reg_v list)
+End
+
+(* An interval of allocated memory.
+ * Args: whether it's freeable, the starting address (inclusive), and the ending address
+ * (exclusive)
+ *)
+Datatype:
+  interval = Interval bool num num
+End
+
+Datatype:
+  heap = <| memory : addr |-> 'a # word8;
+            allocations : interval set;
+            valid_addresses : addr set|>
+End
+
+(* shapes statically describe the shape of a value in a register. Flat shapes
+ * take a given number of bytes, Array shapes are replicated a certain number of
+ * times
+ *)
+Datatype:
+  shape =
+  | Flat num 'a
+  | Array shape num
+  | Tuple (shape list)
+End
+
+(* Does a value have a given shape. The function argument answers the question
+ * for flat values/shapes.
+ * We use mutual recursion instead of list_rel to work around a HOL bug. *)
+Definition value_shape_def:
+  (value_shape f (Flat n t) (FlatV x) ⇔ f n t x) ∧
+  (value_shape f (Array s n) (AggV vs) ⇔
+    every (value_shape f s) vs ∧ length vs = n) ∧
+  (value_shape f (Tuple ss) (AggV vs) ⇔
+    value_shapes f ss vs) ∧
+  (value_shape _ _ _ ⇔ F) ∧
+  (value_shapes f [] [] ⇔ T) ∧
+  (value_shapes f (s::ss) (v::vs) ⇔
+    value_shape f s v ∧ value_shapes f ss vs) ∧
+  (value_shapes _ _ _ ⇔ F)
+Termination
+  WF_REL_TAC `measure (\x. case x of | INL (_, x, _) => shape_size (\x.0) x | INR (_, y, _) => shape1_size (\x.0) y)`
+End
+
+Theorem value_shapes_list_rel:
+  ∀f ss vs. value_shapes f ss vs ⇔ list_rel (value_shape f) ss vs
+Proof
+  Induct_on `ss` >> Cases_on `vs` >> rw [value_shape_def]
+QED
+
+Theorem value_shape_cases:
+  ∀f s v.
+    value_shape f s v ⇔
+      (∃n t x. s = Flat n t ∧ v = FlatV x ∧ f n t x) ∨
+      (∃s2 n vs. s = Array s2 n ∧ v = AggV vs ∧
+        every (value_shape f s2) vs ∧ length vs = n) ∨
+      (∃ss vs. s = Tuple ss ∧ v = AggV vs ∧ value_shapes f ss vs)
+Proof
+  rw [] >>
+  Cases_on `s` >> Cases_on `v` >> rw [value_shape_def] >> metis_tac []
+QED
+
+Definition sizeof_def:
+  (sizeof (Flat n t) = n) ∧
+  (sizeof (Array s n) = n * sizeof s) ∧
+  (sizeof (Tuple ss) = sum (map sizeof ss))
+Termination
+  WF_REL_TAC `measure (shape_size (\x.0))` >> rw [] >>
+  Induct_on `ss` >> rw [definition "shape_size_def"] >>
+  res_tac >> decide_tac
+End
+
+Definition interval_to_set_def:
+  interval_to_set (Interval _ start stop) =
+    { n | start ≤ n ∧ n < stop }
+End
+
+Definition interval_ok_def:
+  interval_ok (Interval b i1 i2) valid_addresses ⇔
+    i1 ≤ i2 ∧ image A (interval_to_set (Interval b i1 i2)) ⊆ valid_addresses
+End
+
+Definition interval_freeable_def:
+  interval_freeable (Interval b _ _) ⇔ b
+End
+
+Definition is_allocated_def:
+  is_allocated b1 h ⇔
+    interval_ok b1 h.valid_addresses ∧
+    ∃b2. b2 ∈ h.allocations ∧ (interval_freeable b1 ⇔ interval_freeable b2) ∧
+         interval_to_set b1 ⊆ interval_to_set b2
+End
+
+Definition is_free_def:
+  is_free b1 h ⇔
+    interval_ok b1 h.valid_addresses ∧
+    ∀b2. b2 ∈ h.allocations ⇒ interval_to_set b1 ∩ interval_to_set b2 = ∅
+End
+
+(* The allocations are of intervals that don't overlap *)
+Definition allocations_ok_def:
+  allocations_ok h ⇔
+    ∀i1 i2.
+      i1 ∈ h.allocations ∧ i2 ∈ h.allocations
+      ⇒
+      interval_ok i1 h.valid_addresses ∧ interval_ok i2 h.valid_addresses ∧
+      (interval_to_set i1 ∩ interval_to_set i2 ≠ ∅ ⇒ i1 = i2)
+End
+
+(* The heap maps exactly the address in the allocations *)
+Definition heap_ok_def:
+  heap_ok h ⇔
+    allocations_ok h ∧
+    ∀n. flookup h.memory (A n) ≠ None ⇔ ∃i. i ∈ h.allocations ∧ n ∈ interval_to_set i
+End
+
+Definition get_bytes_def:
+  get_bytes h (Interval _ start stop) =
+    map
+      (λoff.
+        case flookup h.memory (A (start + off)) of
+        | None => (F, 0w)
+        | Some w => w)
+      (count_list (stop - start))
+End
+
+Definition set_bytes_def:
+  (set_bytes p [] n h = h) ∧
+  (set_bytes p (b::bs) n h =
+    set_bytes p bs (Suc n) (h with memory := h.memory |+ (A n, (p, b))))
+End
+
+(* Allocate a free chunk of memory, and write non-deterministic bytes into it *)
+Inductive allocate:
+   b = Interval T p (p + size) ∧
+   is_free b h ∧
+   length bytes = size
+   ⇒
+   allocate h size tag (w, set_bytes tag bytes p
+                           <| memory := h.memory;
+                              allocations := { b } ∪ h.allocations;
+                              valid_addresses := h.valid_addresses |>)
+End
+
+Definition deallocate_def:
+  deallocate addrs h =
+    let to_remove = { Interval T n stop | A n ∈ set addrs ∧ Interval T n stop ∈ h.allocations } in
+      <| memory := fdiff h.memory (image A (bigunion (image interval_to_set to_remove)));
+         allocations := h.allocations DIFF to_remove;
+         valid_addresses := h.valid_addresses |>
+End
+
+
+(* Read len bytes from the list of bytes, and convert it into a word value,
+ * little-endian encoding *)
+Definition le_read_w_def:
+  le_read_w len (bs : word8 list) =
+    if length bs < len then
+      (l2w 256 (map w2n bs), [])
+    else
+      (l2w 256 (map w2n (take len bs)), drop len bs)
+End
+
+(* Return len bytes that are the little-endian encoding of the argument word *)
+Definition le_write_w_def:
+  le_write_w len w =
+    let (l : word8 list) = map n2w (w2l 256 w) in
+      take len (l ++ replicate (len - length l) 0w)
+End
+
+(* Read a from a list of bytes bs to build a register value described by a
+ * shape. The function f is applied to the word read from a flat list of bytes
+ * in little-endian order. *)
+Definition bytes_to_value_def:
+  (bytes_to_value f (Flat n t) bs = (FlatV o f n t ## I) (le_read_w n bs)) ∧
+  (bytes_to_value f (Array s n) bs = (AggV ## I) (read_array f n s bs)) ∧
+  (bytes_to_value f (Tuple ts) bs = (AggV ## I) (read_str f ts bs)) ∧
+  (read_array f 0 s bs = ([], bs)) ∧
+  (read_array f (Suc n) s bs =
+    let (v, bs) = bytes_to_value f s bs in
+    let (rest, bs) = read_array f n s bs in
+      (v::rest, bs)) ∧
+  (read_str f [] bs = ([], bs)) ∧
+  (read_str f (s::ss) bs =
+    let (v, bs) = bytes_to_value f s bs in
+    let (rest, bs) = read_str f ss bs in
+      (v::rest, bs))
+Termination
+  WF_REL_TAC `measure (λx. case x of
+                           | INL (_, t, bs) => shape_size (\x.0) t
+                           | INR (INL (_, n, t, bs)) => n + shape_size (\x.0) t
+                           | INR (INR (_, ts, bs)) => shape1_size (\x.0) ts)`
+End
+
+(* Convert the given value to a list of bytes, the function gives the size, and
+ * a machine word for a flat value *)
+Definition value_to_bytes_def:
+  (value_to_bytes f (FlatV x) =
+    let (size, word) = f x in
+      le_write_w size word) ∧
+  (value_to_bytes f (AggV vs) = flat (map (value_to_bytes f) vs))
+Termination
+  WF_REL_TAC `measure (reg_v_size (\x. 0) o snd)` >>
+  Induct >> rw [definition "reg_v_size_def"] >>
+  TRY (first_x_assum drule) >>
+  decide_tac
+End
+
+(* ----- Theorems about converting between values and byte lists ----- *)
+
+Theorem le_write_w_length:
+  ∀l x. length (le_write_w l w) = l
+Proof
+  rw [le_write_w_def]
+QED
+
+Theorem v2b_size_lem:
+  (∀(f:num->'a->'b->bool) s v. (∀n t x. f n t x ⇒ fst (g x) = n) ∧ value_shape f s v ⇒ length (value_to_bytes g v) = sizeof s) ∧
+  (∀(f:num->'a->'b->bool) ss vs. (∀n t x. f n t x ⇒ fst (g x) = n) ∧ value_shapes f ss vs ⇒ sum (map (length o value_to_bytes g) vs) = sum (map sizeof ss))
+Proof
+  ho_match_mp_tac value_shape_ind >>
+  rw [value_to_bytes_def, sizeof_def, value_shape_def]
+  >- (
+    pairarg_tac >> simp [] >>
+    metis_tac [FST, le_write_w_length])
+  >- (
+    simp [LENGTH_FLAT, MAP_MAP_o, combinTheory.o_DEF] >>
+    Induct_on `vs` >> rw [ADD1] >> fs [LEFT_ADD_DISTRIB] >>
+    metis_tac [])
+  >- (fs [LENGTH_FLAT, ETA_THM, MAP_MAP_o, combinTheory.o_DEF] >> metis_tac [])
+  >- metis_tac [ADD_COMM]
+QED
+
+Theorem v2b_size:
+  ∀f s v g. (∀n t x. f n t x ⇒ fst (g x) = n) ∧ value_shape f s v ⇒ length (value_to_bytes g v) = sizeof s
+Proof
+  metis_tac [v2b_size_lem]
+QED
+
+Theorem b2v_size_lem:
+  (∀(f:num->'c ->'a word -> 'b) s bs. sizeof s ≤ length bs ⇒
+    ∃v. bytes_to_value f s bs = (v, drop (sizeof s) bs)) ∧
+  (∀(f:num->'c ->'a word -> 'b) n s bs. n * sizeof s ≤ length bs ⇒
+    ∃vs. read_array f n s bs = (vs, drop (n * sizeof s) bs)) ∧
+  (∀(f:num->'c ->'a word -> 'b) ss bs. sum (map sizeof ss) ≤ length bs ⇒
+    ∃vs. read_str f ss bs = (vs, drop (sum (map sizeof ss)) bs))
+Proof
+  ho_match_mp_tac bytes_to_value_ind >>
+  rw [sizeof_def, bytes_to_value_def, le_read_w_def] >>
+  fs []
+  >- (simp [PAIR_MAP] >> metis_tac [SND])
+  >- (
+    pairarg_tac >> rw [] >> pairarg_tac >> rw [] >>
+    fs [ADD1] >> rw [] >> fs [DROP_DROP_T, LEFT_ADD_DISTRIB])
+  >- fs [DROP_DROP_T, LEFT_ADD_DISTRIB]
+QED
+
+Theorem b2v_size:
+  ∀f s bs. sizeof s ≤ length bs ⇒
+    ∃v. bytes_to_value f s bs = (v, drop (sizeof s) bs)
+Proof
+  metis_tac [b2v_size_lem]
+QED
+
+Theorem b2v_smaller:
+  ∀f s bs. sizeof s ≤ length bs ⇒
+    length (snd (bytes_to_value f s bs)) = length bs - sizeof s
+Proof
+  rw [] >> imp_res_tac b2v_size >>
+  Cases_on `bytes_to_value f s bs` >> fs [] >>
+  first_x_assum (qspec_then `f` mp_tac) >> rw []
+QED
+
+Theorem b2v_append_lem:
+  (∀(f:num->'c->'a word -> 'b) s bs. sizeof s ≤ length bs ⇒
+    bytes_to_value f s (bs ++ bs') = (I ## (λx. x ++ bs')) (bytes_to_value f s bs)) ∧
+  (∀(f:num->'c->'a word -> 'b) n s bs. n * sizeof s ≤ length bs ⇒
+    ∃vs. read_array f n s (bs ++ bs') = (I ## (λx. x ++ bs')) (read_array f n s bs)) ∧
+  (∀(f:num->'c->'a word -> 'b) ss bs. sum (map sizeof ss) ≤ length bs ⇒
+    ∃vs. read_str f ss (bs ++ bs') = (I ## (λx. x ++ bs')) (read_str f ss bs))
+Proof
+  ho_match_mp_tac bytes_to_value_ind >>
+  rw [sizeof_def, bytes_to_value_def, le_read_w_def] >>
+  fs [TAKE_APPEND, DROP_APPEND,
+      DECIDE ``!x y. x ≤ y ⇒ x - y = 0n``, ETA_THM]
+  >- (simp [PAIR_MAP] >> metis_tac [SND])
+  >- (simp [PAIR_MAP] >> metis_tac [SND])
+  >- (
+    rpt (pairarg_tac >> simp []) >> fs [ADD1] >>
+    BasicProvers.VAR_EQ_TAC >> fs [LEFT_ADD_DISTRIB] >>
+    first_x_assum irule >>
+    `sizeof s ≤ length bs` by decide_tac >>
+    qspec_then `f` drule b2v_smaller >>
+    disch_then (qspec_then `f` mp_tac) >>
+    rw [])
+  >- (
+    rpt (pairarg_tac >> simp []) >> fs [ADD1] >>
+    BasicProvers.VAR_EQ_TAC >> fs [LEFT_ADD_DISTRIB] >>
+    first_x_assum irule >>
+    `sizeof s ≤ length bs` by decide_tac >>
+    qspec_then `f` drule b2v_smaller >>
+    disch_then (qspec_then `f` mp_tac) >>
+    rw [])
+QED
+
+Theorem b2v_append:
+  ∀f s bs bs'. sizeof s ≤ length bs ⇒
+    bytes_to_value f s (bs ++ bs') = (I ## (λx. x ++ bs')) (bytes_to_value f s bs)
+Proof
+  metis_tac [b2v_append_lem]
+QED
+
+Theorem le_read_write:
+  ∀n w bs.
+    w2n w < 256 ** n ⇒ le_read_w n (le_write_w n w ⧺ bs) = (w, bs)
+Proof
+  rw [le_read_w_def, le_write_w_length]
+  >- (
+    `take n (le_write_w n w ⧺ bs) = le_write_w n w`
+    by metis_tac [le_write_w_length, TAKE_LENGTH_APPEND] >>
+    simp [le_write_w_def, w2l_def, l2w_def] >>
+    Cases_on `w` >> simp [] >> fs [l2n_padding, TAKE_APPEND, take_replicate] >>
+    simp [MAP_TAKE, MAP_MAP_o, combinTheory.o_DEF, mod_n2l] >>
+    rename1 `n2l 256 m` >>
+    Cases_on `n = 0` >> fs [] >>
+    `length (n2l 256 m) ≤ n`
+    by (
+      rw [LENGTH_n2l] >>
+      `256 = 2 ** 8` by EVAL_TAC >>
+      ASM_REWRITE_TAC [] >> simp [log_change_base_power, GSYM LESS_EQ] >>
+      `n2w m ≠ 0w` by simp [] >>
+      rw [] >> fs [bitTheory.LOG2_def, dimword_def] >>
+      `8 * (log 2 m DIV 8) ≤ log 2 m` by metis_tac [mul_div_bound, EVAL ``8 ≠ 0n``] >>
+      `LOG 2 m ≤ LOG 2 (256 ** n)` by simp [LOG_LE_MONO] >>
+      pop_assum mp_tac >>
+      `256 = 2 ** 8` by EVAL_TAC >>
+      ASM_REWRITE_TAC [EXP_MUL] >> simp [log_base_power] >>
+      Cases_on `log 2 m DIV 8 = n` >> rw [] >>
+      CCONTR_TAC >> fs [] >>
+      `log 2 m = (8 * (log 2 m DIV 8))` by intLib.COOPER_TAC >> fs [] >>
+      `2 ** log 2 m = 2 ** (8 * (log 2 m DIV 8))` by rw [] >>
+      fs [EXP_EXP_MULT] >>
+      `2 ** log 2 m ≤ m` by rw [exp_log_bound] >>
+      decide_tac) >>
+    simp [mod_n2l, l2n_n2l, TAKE_LENGTH_TOO_LONG])
+  >- metis_tac [le_write_w_length, DROP_LENGTH_APPEND]
+QED
+
+Theorem le_write_read:
+  ∀n w bs bs'.
+    256 ** n ≤ dimword (:'a) ∧
+    n ≤ length bs ∧
+    le_read_w n bs = (w:'a word, bs')
+    ⇒
+    le_write_w n w ++ bs' = bs
+Proof
+  rw [le_read_w_def] >>
+  qmatch_goalsub_abbrev_tac `l2w _ l` >>
+  `le_write_w n (l2w 256 l) = take n bs` suffices_by metis_tac [TAKE_DROP] >>
+  simp [le_write_w_def, w2l_l2w] >>
+  `l2n 256 l < 256 ** n`
+  by (
+    `n ≤ length bs` by decide_tac >>
+    metis_tac [l2n_lt, LENGTH_TAKE, LENGTH_MAP, EVAL ``0n < 256``]) >>
+  fs [] >>
+  `every ($> 256) l`
+  by (
+    simp [EVERY_MAP, Abbr `l`] >> irule EVERY_TAKE >> simp [] >>
+    rpt (pop_assum kall_tac) >>
+    Induct_on `bs` >> rw [] >>
+    Cases_on `h` >> fs []) >>
+  rw [n2l_l2n]
+  >- (
+    rw [TAKE_def, take_replicate] >>
+    Cases_on `n` >> fs [] >>
+    rfs [l2n_0] >> unabbrev_all_tac >> fs [EVERY_MAP] >>
+    ONCE_REWRITE_TAC [GSYM REPLICATE] >>
+    qmatch_goalsub_abbrev_tac `take n _` >>
+    qpat_assum `¬(_ < _)` mp_tac >>
+    qpat_assum `every (\x. 0 = w2n x) _` mp_tac >>
+    rpt (pop_assum kall_tac) >>
+    qid_spec_tac `bs` >>
+    Induct_on `n` >> rw [] >>
+    Cases_on `bs` >> rw [] >> fs [] >>
+    Cases_on `h` >> fs [] >>
+    first_x_assum irule >> rw [] >>
+    irule MONO_EVERY >>
+    qexists_tac `(λx. 0 = w2n x)` >> rw []) >>
+  fs [MAP_TAKE, MAP_MAP_o, combinTheory.o_DEF] >>
+  `exists (\y. 0 ≠ y) l`
+  by (
+    fs [l2n_eq_0, combinTheory.o_DEF] >> fs [EXISTS_MEM, EVERY_MEM] >>
+    qexists_tac `x` >> rfs [MOD_MOD, GREATER_DEF]) >>
+  simp [LOG_l2n_dropWhile] >>
+  `length (dropWhile ($= 0) (reverse l)) ≠ 0`
+  by (
+    Cases_on `l` >> fs [dropWhile_eq_nil, combinTheory.o_DEF, EXISTS_REVERSE]) >>
+  `0 < length (dropWhile ($= 0) (reverse l))` by decide_tac >>
+  fs [SUC_PRE] >>
+  `map n2w l = take n bs`
+  by (simp [Abbr `l`, MAP_TAKE, MAP_MAP_o, combinTheory.o_DEF, n2w_w2n]) >>
+  simp [TAKE_TAKE_MIN] >>
+  `length l = n` by simp [Abbr `l`] >>
+  `length (dropWhile ($= 0) (reverse l)) ≤ n`
+  by metis_tac [LESS_EQ_TRANS, LENGTH_dropWhile_LESS_EQ, LENGTH_REVERSE] >>
+  rw [MIN_DEF] >> fs []
+  >- (
+    simp [TAKE_APPEND, TAKE_TAKE_MIN, MIN_DEF, take_replicate] >>
+    `replicate (length l − length (dropWhile ($= 0) (reverse l))) 0w =
+     take (length l − (length (dropWhile ($= 0) (reverse l)))) (drop (length (dropWhile ($= 0) (reverse l))) bs)`
+    suffices_by (rw [] >> irule take_drop_partition >> simp []) >>
+    rw [LIST_EQ_REWRITE, EL_REPLICATE, EL_TAKE, EL_DROP] >>
+   `length (dropWhile ($= 0) (reverse l)) =
+     length (dropWhile (λx. 0 = w2n x) (reverse (take (length l) bs)))`
+    by (
+      `reverse l = reverse (take (length l) (map w2n bs))` by metis_tac [] >>
+      ONCE_ASM_REWRITE_TAC [] >>
+      qpat_x_assum `Abbrev (l = _)` kall_tac >>
+      simp [GSYM MAP_TAKE, GSYM MAP_REVERSE, dropWhile_map, combinTheory.o_DEF]) >>
+    fs [] >>
+    `x + length (dropWhile (λx. 0 = w2n x) (reverse (take (length l) bs))) < length l` by decide_tac >>
+    drule (SIMP_RULE std_ss [LET_THM] dropWhile_rev_take) >>
+    rw [] >>
+    REWRITE_TAC [GSYM w2n_11, word_0_n2w] >>
+    simp [])
+  >- rw [TAKE_APPEND, TAKE_TAKE]
+QED
+
+Theorem b2v_v2b_lem:
+  (∀f s v.
+    value_shape f s v ⇒
+    (∀x t n. f n t x ⇒ fst (h x) = n ∧ g n t (snd (h x)) = x ∧ w2n (snd (h x)) < 256 ** n) ⇒
+    ∀bs.
+      bytes_to_value (g:num -> 'c -> 'a word -> 'b) s (value_to_bytes h v ++ bs) = (v, bs)) ∧
+  (∀f ss vs.
+    value_shapes f ss vs ⇒
+    (∀x t n. f n t x ⇒ fst (h x) = n ∧ g n t (snd (h x)) = x ∧ w2n (snd (h x)) < 256 ** n) ⇒
+    ∀bs.
+      read_str (g:num -> 'c -> 'a word -> 'b) ss (flat (map (value_to_bytes h) vs) ++ bs) = (vs, bs))
+Proof
+  ho_match_mp_tac value_shape_ind >> rw [value_shape_def] >>
+  fs [bytes_to_value_def, value_to_bytes_def] >> rw []
+  >- (
+    pairarg_tac >> fs [] >>
+    first_x_assum drule >> simp [] >> rw [] >>
+    simp [le_read_write])
+  >- (
+    qmatch_abbrev_tac `_ x = _` >>
+    `x = (vs, bs)` suffices_by (simp [PAIR_MAP] >> metis_tac [PAIR_EQ, FST, SND]) >>
+    unabbrev_all_tac >>
+    qid_spec_tac `bs` >> Induct_on `vs` >> simp [bytes_to_value_def] >>
+    rw [] >> fs [definition "reg_v_size_def"] >>
+    pairarg_tac >> fs [] >>
+    pairarg_tac >> fs [] >>
+    rename1 `value_shape _ s v1` >>
+    qpat_x_assum `_ ⇒ !bs. P bs` mp_tac >> impl_tac >> simp [] >>
+    metis_tac [APPEND_ASSOC, PAIR_EQ])
+  >- (
+    qmatch_abbrev_tac `_ x = _` >>
+    `x = (vs, bs)` suffices_by (simp [PAIR_MAP] >> metis_tac [PAIR_EQ, FST, SND]) >>
+    metis_tac [])
+  >- (
+    pairarg_tac >> fs [] >>
+    pairarg_tac >> fs [] >>
+    metis_tac [APPEND_ASSOC, PAIR_EQ])
+QED
+
+Theorem b2v_v2b:
+  ∀f g h s v bs.
+    value_shape f s v ⇒
+    (∀x n t. f n t x ⇒ fst (h x) = n ∧ g n t (snd (h x)) = x ∧ w2n (snd (h x)) < 256 ** n) ⇒
+      bytes_to_value g s (value_to_bytes h v ++ bs) = (v, bs)
+Proof
+  metis_tac [b2v_v2b_lem]
+QED
+
+Theorem flookup_set_bytes:
+  ∀tag bytes n h n'.
+    flookup ((set_bytes tag bytes n h).memory) (A n') =
+      if n ≤ n' ∧ n' < n + length bytes then
+        Some (tag, el (n' - n) bytes)
+      else
+        flookup h.memory (A n')
+Proof
+  Induct_on `bytes` >> rw [set_bytes_def, EL_CONS, PRE_SUB1] >>
+  fs [ADD1, FLOOKUP_UPDATE] >>
+  `n = n'` by decide_tac >>
+  rw []
+QED
+
+Theorem set_bytes_unchanged:
+  ∀t bs p h. (set_bytes t bs p h).valid_addresses = h.valid_addresses ∧
+             (set_bytes t bs p h).allocations = h.allocations
+Proof
+  Induct_on `bs` >> rw [set_bytes_def]
+QED
+
+Theorem allocate_unchanged:
+  ∀h1 v1 t h2 v2.
+    allocate h1 v1 t (v2, h2)
+    ⇒
+    h1.valid_addresses = h2.valid_addresses ∧
+    h1.allocations ⊆ h2.allocations
+Proof
+  rw [allocate_cases] >> rw [set_bytes_unchanged]
+QED
+
+Theorem allocate_heap_ok:
+  ∀h1 v1 t v2 h2. heap_ok h1 ∧ allocate h1 v1 t (v2,h2) ⇒ heap_ok h2
+Proof
+  rw [allocate_cases, heap_ok_def]
+  >- (
+    fs [allocations_ok_def] >> rpt gen_tac >> disch_tac >> fs [is_free_def] >> rw [] >>
+    fs [set_bytes_unchanged] >> metis_tac [INTER_COMM])
+  >- (
+    rw [flookup_set_bytes, set_bytes_unchanged]
+    >- rw [RIGHT_AND_OVER_OR, EXISTS_OR_THM, interval_to_set_def] >>
+    eq_tac >> rw [] >> fs [interval_to_set_def] >>
+    metis_tac [])
+QED
+
+Theorem set_bytes_heap_ok:
+  ∀h tag bytes n b.
+    heap_ok h ∧ is_allocated (Interval b n (n + length bytes)) h
+    ⇒
+    heap_ok (set_bytes tag bytes n h)
+Proof
+  rw [heap_ok_def]
+  >- (fs [allocations_ok_def] >> rw [set_bytes_unchanged] >> metis_tac [])
+  >- (
+    fs [flookup_set_bytes, set_bytes_unchanged] >> rw [] >>
+    fs [is_allocated_def, interval_to_set_def, SUBSET_DEF] >>
+    metis_tac [LESS_EQ_REFL, DECIDE ``!x y. x < x + SUC y``])
+QED
+
+export_theory ();
