sledge/semantics/miscScript.sml
@@ -1,0 +1,172 @@
+(*
+ * Copyright (c) Facebook, Inc. and its affiliates.
+ *
+ * This source code is licensed under the MIT license found in the
+ * LICENSE file in the root directory of this source tree.
+ *)
+
+(* Misc. theorems that aren't specific to the semantics of LLVM or Sledge. These
+ * could be upstreamed to HOL, and should eventually. *)
+
+open HolKernel boolLib bossLib Parse;
+open listTheory rich_listTheory arithmeticTheory wordsTheory;
+open finite_mapTheory open logrootTheory numposrepTheory;
+open settingsTheory;
+
+new_theory "misc";
+
+numLib.prefer_num ();
+
+(* ----- Theorems about list library functions ----- *)
+
+Theorem dropWhile_map:
+  ∀P f l. dropWhile P (map f l) = map f (dropWhile (P o f) l)
+Proof
+  Induct_on `l` >> rw []
+QED
+
+Theorem dropWhile_prop:
+  ∀P l x. x < length l - length (dropWhile P l) ⇒ P (el x l)
+Proof
+  Induct_on `l` >> rw [] >>
+  Cases_on `x` >> fs []
+QED
+
+Theorem dropWhile_rev_take:
+  ∀P n l x.
+    let len = length (dropWhile P (reverse (take n l))) in
+      x + len < n ∧ n ≤ length l ⇒ P (el (x + len) l)
+Proof
+  rw [] >>
+  `P (el ((n - 1 - x - length (dropWhile P (reverse (take n l))))) (reverse (take n l)))`
+  by (irule dropWhile_prop >> simp [LENGTH_REVERSE]) >>
+  rfs [EL_REVERSE, EL_TAKE, PRE_SUB1]
+QED
+
+Theorem take_replicate:
+  ∀m n x. take m (replicate n x) = replicate (min m n) x
+Proof
+  Induct_on `n` >> rw [TAKE_def, MIN_DEF] >> fs [] >>
+  Cases_on `m` >> rw []
+QED
+
+Theorem length_take_less_eq:
+  ∀n l. length (take n l) ≤ n
+Proof
+  Induct_on `l` >> rw [TAKE_def] >>
+  Cases_on `n` >> fs []
+QED
+
+Theorem flat_drop:
+  ∀n m ls. flat (drop m ls) = drop (length (flat (take m ls))) (flat ls)
+Proof
+  Induct_on `ls` >> rw [DROP_def, DROP_APPEND] >>
+  irule (GSYM DROP_LENGTH_TOO_LONG) >> simp []
+QED
+
+Theorem take_is_prefix:
+  ∀n l. take n l ≼ l
+Proof
+  Induct_on `l` >> rw [TAKE_def]
+QED
+
+Theorem sum_prefix:
+  ∀l1 l2. l1 ≼ l2 ⇒ sum l1 ≤ sum l2
+Proof
+  Induct >> rw [] >> Cases_on `l2` >> fs []
+QED
+
+Theorem flookup_fdiff:
+  ∀m s k.
+    flookup (fdiff m s) k =
+      if k ∈ s then None else flookup m k
+Proof
+  rw [FDIFF_def, FLOOKUP_DRESTRICT] >> fs []
+QED
+
+(* ----- Theorems about log ----- *)
+
+Theorem mul_div_bound:
+  ∀m n. n ≠ 0 ⇒ m - (n - 1) ≤ n * (m DIV n) ∧ n * (m DIV n) ≤ m
+Proof
+  rw [] >>
+  `0 < n` by decide_tac >>
+  drule DIVISION >> disch_then (qspec_then `m` mp_tac) >>
+  decide_tac
+QED
+
+Theorem exp_log_bound:
+  ∀b n. 1 < b ∧ n ≠ 0 ⇒ n DIV b + 1 ≤ b ** (log b n) ∧ b ** (log b n) ≤ n
+Proof
+  rw [] >> `0 < n` by decide_tac >>
+  drule LOG >> disch_then drule >> rw [] >>
+  fs [ADD1, EXP_ADD] >>
+  simp [DECIDE ``∀x y. x + 1 ≤ y ⇔ x < y``] >>
+  `∃x. b = Suc x` by intLib.COOPER_TAC >>
+  `b * (n DIV b) < b * b ** log b n` suffices_by metis_tac [LESS_MULT_MONO] >>
+  pop_assum kall_tac >>
+  `b ≠ 0` by decide_tac >>
+  drule mul_div_bound >> disch_then (qspec_then `n` mp_tac) >>
+  decide_tac
+QED
+
+Theorem log_base_power:
+  ∀n b. 1 < b ⇒ log b (b ** n) = n
+Proof
+  Induct >> rw [EXP, LOG_1] >>
+  Cases_on `n` >> rw [LOG_BASE] >>
+  first_x_assum drule >> rw [] >>
+  simp [Once EXP, LOG_MULT]
+QED
+
+Theorem log_change_base_power:
+  ∀m n b. 1 < b ∧ m ≠ 0 ∧ n ≠ 0 ⇒ log (b ** n) m = log b m DIV n
+Proof
+  rw [] >> irule LOG_UNIQUE >>
+  rw [ADD1, EXP_MUL, LEFT_ADD_DISTRIB] >>
+  qmatch_goalsub_abbrev_tac `x DIV _` >>
+  drule mul_div_bound >> disch_then (qspec_then `x` mp_tac) >> rw []
+  >- (
+    irule LESS_LESS_EQ_TRANS >>
+    qexists_tac `b ** (x+1)` >> rw [] >>
+    unabbrev_all_tac >>
+    simp [EXP_ADD] >>
+    `b * (m DIV b + 1) ≤ b * b ** log b m`
+    by metis_tac [exp_log_bound, LESS_MONO_MULT, MULT_COMM] >>
+    `m < b * (m DIV b + 1)` suffices_by decide_tac >>
+    simp [LEFT_ADD_DISTRIB] >>
+    `b ≠ 0` by decide_tac >>
+    `m - (b - 1) ≤ b * (m DIV b)` by metis_tac [mul_div_bound] >>
+    fs [])
+  >- (
+    irule LESS_EQ_TRANS >>
+    qexists_tac `b ** (log b m)` >> rw [] >>
+    unabbrev_all_tac >>
+    metis_tac [exp_log_bound])
+QED
+
+(* ----- Theorems about word stuff ----- *)
+
+Theorem l2n_padding:
+  ∀ws n. l2n 256 (ws ++ map w2n (replicate n 0w)) = l2n 256 ws
+Proof
+  Induct >> rw [l2n_def] >>
+  Induct_on `n` >> rw [l2n_def]
+QED
+
+Theorem l2n_0:
+  ∀l b. b ≠ 0 ∧ every ($> b)  l⇒ (l2n b l = 0 ⇔ every ($= 0) l)
+Proof
+  Induct >> rw [l2n_def] >>
+  eq_tac >> rw []
+QED
+
+Theorem mod_n2l:
+  ∀d n. 0 < d ⇒ map (\x. x MOD d) (n2l d n) = n2l d n
+Proof
+  rw [] >> drule n2l_BOUND >> disch_then (qspec_then `n` mp_tac) >>
+  qspec_tac (`n2l d n`, `l`) >>
+  Induct >> rw []
+QED
+
+export_theory ();
